example/ToyExamplesBlocks.thy
@@ -6,7 +6,7 @@ begin
 lemmas evm_fun_simps = 
   stack_inst_code.simps inst_size_def inst_code.simps 
 
-lemmas cfg_simps = build_cfg_def byteListInt_def find_block_def extract_indexes_def build_basic_blocks_def
+lemmas blocks_simps = build_blocks_def byteListInt_def find_block_def extract_indexes_def build_vertices_def
  aux_basic_block.simps add_address_def block_pt_def
 
 lemmas word_rcat_simps = word_rcat_def bin_rcat_def
@@ -24,11 +24,11 @@ by (rule ext, simp add: pure_def sep_conj_def emp_def )+
 (* Example with a Jumpi and a No block *)
 
 definition c where
-"c = build_cfg [ Stack (PUSH_N [1]), Stack (PUSH_N [8]), Pc JUMPI, Stack (PUSH_N [1]), Misc STOP, Pc JUMPDEST, Stack (PUSH_N [2]), Misc STOP]"
+"c = build_blocks [ Stack (PUSH_N [1]), Stack (PUSH_N [8]), Pc JUMPI, Stack (PUSH_N [1]), Misc STOP, Pc JUMPDEST, Stack (PUSH_N [2]), Misc STOP]"
 
 schematic_goal c_val:
  " c = ?p"
- by(simp add: c_def  word_rcat_simps Let_def evm_fun_simps dropWhile.simps  cfg_simps next_i_def
+ by(simp add: c_def  word_rcat_simps Let_def evm_fun_simps dropWhile.simps  blocks_simps next_i_def
   split:if_splits nat.splits option.splits )
 
 context
@@ -40,14 +40,14 @@ begin
 (* Should not apply any auto. Otherwise, auto simplify with "cond=0" even when it is wrong *)
 (* For a jumpif that can be solved statically, it works *)
 lemma
- "\<exists>rest. triple_cfg c
+ "\<exists>rest. triple_blocks c
 (continuing ** stack_height 0 ** program_counter 0 ** gas_pred 1000 ** memory_usage 0)
-(0,the (cfg_blocks c 0))
+(0,the (blocks_list c 0))
 (stack 0 (word_rcat [2::byte]) ** rest)"
  apply(unfold c_val)
  apply (simp)
  apply(rule exI)
- apply(rule cfg_jumpi[where rest=emp])
+ apply(rule blocks_jumpi[where rest=emp])
         apply(simp)
        prefer 4
        apply(simp)
@@ -81,7 +81,7 @@ lemma
   apply(simp add: word_rcat_simps)
   prefer 2
   apply(simp add: word_rcat_simps)
- apply(rule cfg_no)
+ apply(rule blocks_no)
  apply(rule seq_inst)
   apply(rule inst_strengthen_pre[OF inst_jumpdest[where rest=emp]])
   apply(rule impI)
@@ -111,23 +111,23 @@ done
 (* Same example but we put an unknown value and an if in the post condition *)
 (* For a jumpif where we don't know at all which branch to follow, it works *)
 definition c2 where
-"c2 x = build_cfg [ Stack (PUSH_N [x]), Stack (PUSH_N [8]), Pc JUMPI, Stack (PUSH_N [1]), Misc STOP, Pc JUMPDEST, Stack (PUSH_N [2]), Misc STOP]"
+"c2 x = build_blocks [ Stack (PUSH_N [x]), Stack (PUSH_N [8]), Pc JUMPI, Stack (PUSH_N [1]), Misc STOP, Pc JUMPDEST, Stack (PUSH_N [2]), Misc STOP]"
 
 schematic_goal c2_val:
  " c2 x = ?p"
- by(simp add: c2_def  word_rcat_simps Let_def dropWhile.simps cfg_simps next_i_def
+ by(simp add: c2_def  word_rcat_simps Let_def dropWhile.simps blocks_simps next_i_def
   split:if_splits nat.splits option.splits )
 
 lemma
- " \<exists>rest0 restn0. triple_cfg (c2 cond)
+ " \<exists>rest0 restn0. triple_blocks (c2 cond)
 (continuing ** stack_height 0 ** program_counter 0 ** gas_pred 1000 ** memory_usage 0)
-(0, the (cfg_blocks (c2 cond) 0))
+(0, the (blocks_list (c2 cond) 0))
 (if word_rcat [cond] = (0::256 word) then stack 0 (word_rcat [1::byte]) ** restn0 else stack 0 (word_rcat [2::byte]) ** rest0)
 "
 apply(unfold c2_val)
 apply (simp)
 apply(rule exI)+
- apply(rule cfg_jumpi[where rest=emp])
+ apply(rule blocks_jumpi[where rest=emp])
         apply(simp)
        prefer 4
        apply(simp)
@@ -161,7 +161,7 @@ apply(rule exI)+
   apply(simp add: word_rcat_simps)
   prefer 2
   apply(simp add: word_rcat_simps)
- apply(rule cfg_no)
+ apply(rule blocks_no)
   apply(rule seq_inst)
    apply(rule inst_strengthen_pre[OF inst_push_n[where rest=emp]]; rule impI)
    apply(simp)
@@ -175,7 +175,7 @@ apply(rule exI)+
   apply(rule seq_empty; rule impI)
   apply(simp add: word_rcat_simps)
   apply(sep_cancel)
- apply(rule cfg_no)
+ apply(rule blocks_no)
  apply(rule seq_inst)
   apply(rule inst_strengthen_pre[OF inst_jumpdest[where rest=emp]])
   apply(rule impI)
@@ -201,16 +201,16 @@ done
 (* Same example as the previous one but with the unknown value as a precondition *)
 
 lemma
- "\<exists>rest. triple_cfg (c2 cond)
+ "\<exists>rest. triple_blocks (c2 cond)
 (continuing ** stack_height 0 ** program_counter 0 ** gas_pred 1000 ** memory_usage 0 **
  \<langle> (word_rcat [cond] \<noteq> (0::256 word)) \<rangle>)
-(0,the (cfg_blocks (c2 cond) 0))
+(0,the (blocks_list (c2 cond) 0))
 (stack 0 (word_rcat [2::byte]) ** rest )
 "
 apply(unfold c2_val)
 apply (simp)
 apply(rule exI)
-apply(rule cfg_jumpi[where rest="\<langle>word_rcat [cond] \<noteq> (0::256 word)\<rangle>"])
+apply(rule blocks_jumpi[where rest="\<langle>word_rcat [cond] \<noteq> (0::256 word)\<rangle>"])
         apply(simp)
        prefer 4
        apply(simp)
@@ -239,9 +239,9 @@ apply(rule cfg_jumpi[where rest="\<langle>word_rcat [cond] \<noteq> (0::256 word
   apply(simp add: word_rcat_simps)
   prefer 2
   apply(simp add: word_rcat_simps pure_false_simps)
-  apply(rule cfg_no)
+  apply(rule blocks_no)
   apply(rule seq_false_pre)
- apply(rule cfg_no)
+ apply(rule blocks_no)
  apply(rule seq_inst)
   apply(rule inst_strengthen_pre[OF inst_jumpdest[where rest="\<langle>word_rcat [cond] \<noteq> (0::256 word)\<rangle>"]])
   apply(rule impI)
@@ -271,23 +271,23 @@ done
 (* Example with a Jump and a Next block*)
 
 definition c4 where
-"c4 = build_cfg [ Stack (PUSH_N [1]), Stack (PUSH_N [5]), Pc JUMP, Pc JUMPDEST, Stack (PUSH_N [2]), Pc JUMPDEST, Misc STOP]"
+"c4 = build_blocks [ Stack (PUSH_N [1]), Stack (PUSH_N [5]), Pc JUMP, Pc JUMPDEST, Stack (PUSH_N [2]), Pc JUMPDEST, Misc STOP]"
 
 schematic_goal c4_val:
  " c4  = ?p"
- by(simp add: c4_def  word_rcat_simps Let_def dropWhile.simps cfg_simps next_i_def
+ by(simp add: c4_def  word_rcat_simps Let_def dropWhile.simps blocks_simps next_i_def
   split:if_splits nat.splits option.splits )
 
 lemma
- "\<exists>rest. triple_cfg c4
+ "\<exists>rest. triple_blocks c4
 (continuing ** stack_height 0 ** program_counter 0 ** gas_pred 1000 ** memory_usage 0)
-(0, the (cfg_blocks c4 0))
+(0, the (blocks_list c4 0))
 (stack 0 (word_rcat [1::byte]) ** stack_height (Suc (Suc 0)) ** stack 1 (word_rcat [2::byte]) ** rest)
 "
 apply(unfold c4_val)
 apply (simp)
 apply(rule exI)
-apply(rule cfg_jump[where rest="stack 0 (word_rcat [1])"])
+apply(rule blocks_jump[where rest="stack 0 (word_rcat [1])"])
      prefer 3
      apply(simp)
      apply(rule seq_inst)
@@ -317,7 +317,7 @@ apply(rule cfg_jump[where rest="stack 0 (word_rcat [1])"])
      apply(sep_cancel)+
      apply(sep_simp simp: stack_sep; simp add: word_rcat_def stack_def)
     apply(simp add: bin_rcat_def)+
- apply(rule cfg_next)
+ apply(rule blocks_next)
     apply(simp)
    apply(simp)
   apply(rule seq_inst)
@@ -331,7 +331,7 @@ apply(rule cfg_jump[where rest="stack 0 (word_rcat [1])"])
   apply(rule seq_empty; rule impI)
   apply(simp)
   apply(sep_cancel)
- apply(rule cfg_no)
+ apply(rule blocks_no)
  apply(rule seq_inst)
   apply(rule inst_strengthen_pre[OF inst_jumpdest[where rest="stack 0 (word_rcat [1]) \<and>* stack (Suc 0) (word_rcat [2])"]])
   apply(rule impI)
